Reforming basic algorithm on multisets

Worklist_Subsumption1.thy
@@ -1,31 +1,11 @@
 (* Authors: Lammich, Wimmer *)
-section \<open>Generic Worklist Algorithm with Subsumption\<close>
 theory Worklist_Subsumption1
-  imports "../Sepref"
+  imports Worklist_Subsumption_Multiset
 begin
 
-subsection \<open>Utilities\<close>
-definition take_from_set where
-  "take_from_set s = ASSERT (s \<noteq> {}) \<then> SPEC (\<lambda> (x, s'). x \<in> s \<and> s' = s - {x})"
+subsection \<open>From Multisets to Lists\<close>
 
-lemma take_from_set_correct:
-  assumes "s \<noteq> {}"
-  shows "take_from_set s \<le> SPEC (\<lambda> (x, s'). x \<in> s \<and> s' = s - {x})"
-using assms unfolding take_from_set_def by simp
-
-lemmas [refine_vcg] = take_from_set_correct[THEN order.trans]
-
-
-
-definition take_from_mset where
-  "take_from_mset s = ASSERT (s \<noteq> {#}) \<then> SPEC (\<lambda> (x, s'). x \<in># s \<and> s' = s - {#x#})"
-
-lemma take_from_mset_correct:
-  assumes "s \<noteq> {#}"
-  shows "take_from_mset s \<le> SPEC (\<lambda> (x, s'). x \<in># s \<and> s' = s - {#x#})"
-using assms unfolding take_from_mset_def by simp
-
-lemmas [refine_vcg] = take_from_mset_correct[THEN order.trans]
+subsubsection \<open>Utilities\<close>
 
 definition take_from_list where
   "take_from_list s = ASSERT (s \<noteq> []) \<then> SPEC (\<lambda> (x, s'). s = x # s')"
@@ -38,89 +18,25 @@ using assms unfolding take_from_list_def by simp
 lemmas [refine_vcg] = take_from_list_correct[THEN order.trans]
 
 
-lemma set_mset_mp: "set_mset m \<subseteq> s \<Longrightarrow> n < count m x \<Longrightarrow> x\<in>s"
-  by (meson count_greater_zero_iff le_less_trans subsetCE zero_le)
-
-lemma pred_not_lt_is_zero: "(\<not> n - Suc 0 < n) \<longleftrightarrow> n=0" by auto
-
-
-subsection \<open>Search Spaces\<close>
-text \<open>
-  A search space consists of a step relation, a start state,
-  a final state predicate, and a subsumption preorder.
-\<close>
-locale Search_Space_Defs =
-  fixes E :: "'a \<Rightarrow> 'a \<Rightarrow> bool" -- \<open>Step relation\<close>
-    and a\<^sub>0 :: 'a                -- \<open>Start state\<close>
-    and F :: "'a \<Rightarrow> bool"      -- \<open>Final states\<close>
-    and subsumes :: "'a \<Rightarrow> 'a \<Rightarrow> bool" (infix "\<preceq>" 50) -- \<open>Subsumption preorder\<close>
-begin
-  definition reachable where
-    "reachable = E\<^sup>*\<^sup>* a\<^sub>0"
-
-  definition "F_reachable \<equiv> \<exists>a. reachable a \<and> F a"
-
-end
-
-text \<open>The set of reachable states must be finite,
-  subsumption must be a preorder, and be compatible with steps and final states.\<close>
-locale Search_Space = Search_Space_Defs +
-  fixes empty :: "'a \<Rightarrow> bool"
-  assumes finite_reachable: "finite {a. reachable a}"
-
-  assumes refl[intro!, simp]: "a \<preceq> a"
-      and trans[trans]: "a \<preceq> b \<Longrightarrow> b \<preceq> c \<Longrightarrow> a \<preceq> c"
-
-  assumes mono:
-      "a \<preceq> b \<Longrightarrow> E a a' \<Longrightarrow> reachable a \<Longrightarrow> reachable b \<Longrightarrow> \<not> empty a \<Longrightarrow> \<exists> b'. E b b' \<and> a' \<preceq> b'"
-      and empty_subsumes: "empty a \<Longrightarrow> a \<preceq> a'"
-      and empty_mono: "\<not> empty a \<Longrightarrow> a \<preceq> b \<Longrightarrow> \<not> empty b"
-      and empty_E: "reachable x \<Longrightarrow> empty x \<Longrightarrow> E x x' \<Longrightarrow> empty x'"
-      and F_mono: "a \<preceq> a' \<Longrightarrow> F a \<Longrightarrow> F a'"
+context Search_Space_Defs
 begin
 
-  lemma start_reachable[intro!, simp]:
-    "reachable a\<^sub>0"
-  unfolding reachable_def by simp
-
-  lemma step_reachable:
-    assumes "reachable a" "E a a'"
-    shows "reachable a'"
-  using assms unfolding reachable_def by simp
-
-
-  lemma finitely_branching:
-    assumes "reachable a"
-    shows "finite (Collect (E a))"
-    by (metis assms finite_reachable finite_subset mem_Collect_eq step_reachable subsetI)
-
-
-
-end
-
-subsection \<open>Worklist Algorithm\<close>
-
-term card
-
-context Search_Space_Defs begin
-  definition "worklist_var = inv_image (finite_psupset (Collect reachable) <*lex*> measure size) (\<lambda> (a, b,c). (a,b))"
-
-  definition "worklist_inv_frontier passed wait =
+  definition "worklist_inv_frontier_list passed wait =
     (\<forall> a \<in> passed. \<forall> a'. E a a' \<longrightarrow> (\<exists> b' \<in> passed \<union> set wait. a' \<preceq> b'))"
 
-  definition "start_subsumed passed wait = (\<exists> a \<in> passed \<union> set wait. a\<^sub>0 \<preceq> a)"
+  definition "start_subsumed_list passed wait = (\<exists> a \<in> passed \<union> set wait. a\<^sub>0 \<preceq> a)"
 
-  definition "worklist_inv \<equiv> \<lambda> (passed, wait, brk).
+  definition "worklist_inv_list \<equiv> \<lambda> (passed, wait, brk).
     passed \<subseteq> Collect reachable \<and>
     (brk \<longrightarrow> (\<exists> f. reachable f \<and> F f)) \<and>
     (\<not> brk \<longrightarrow>
-      worklist_inv_frontier passed wait
+      worklist_inv_frontier_list passed wait
     \<and> (\<forall> a \<in> passed \<union> set wait. \<not> F a)
-    \<and> start_subsumed passed wait
+    \<and> start_subsumed_list passed wait
     \<and> set wait \<subseteq> Collect reachable)
     "
 
-  definition "add_succ_spec wait a \<equiv> SPEC (\<lambda>(wait',brk).
+  definition "add_succ_spec_list wait a \<equiv> SPEC (\<lambda>(wait',brk).
     if \<exists>a'. E a a' \<and> F a' then
       brk
     else
@@ -128,14 +44,14 @@ context Search_Space_Defs begin
       (\<forall> s \<in> set wait \<union> {a' . E a a'}. \<exists> s' \<in> set wait'. s \<preceq> s')
   )"
 
-  definition worklist_algo where
-    "worklist_algo = do
+  definition worklist_algo_list where
+    "worklist_algo_list = do
       {
         if F a\<^sub>0 then RETURN True
         else do {
           let passed = {};
           let wait = [a\<^sub>0];
-          (passed, wait, brk) \<leftarrow> WHILEIT worklist_inv (\<lambda> (passed, wait, brk). \<not> brk \<and> wait \<noteq> [])
+          (passed, wait, brk) \<leftarrow> WHILEIT worklist_inv_list (\<lambda> (passed, wait, brk). \<not> brk \<and> wait \<noteq> [])
             (\<lambda> (passed, wait, brk). do
               {
                 (a, wait) \<leftarrow> take_from_list wait;
@@ -143,7 +59,7 @@ context Search_Space_Defs begin
                 if (\<exists> a' \<in> passed. a \<preceq> a') then RETURN (passed, wait, brk) else
                 do
                   {
-                    (wait,brk) \<leftarrow> add_succ_spec wait a;
+                    (wait,brk) \<leftarrow> add_succ_spec_list wait a;
                     let passed = insert a passed;
                     RETURN (passed, wait, brk)
                   }
@@ -155,206 +71,45 @@ context Search_Space_Defs begin
       }
     "
 
-end
+end -- \<open>Search Space Defs\<close>
 
-subsubsection \<open>Correctness Proof\<close>
+context Search_Space
+begin
 
-context Search_Space begin
-
-  lemma wf_worklist_var:
-    "wf worklist_var"
-  unfolding worklist_var_def by (auto simp: finite_reachable)
-
-  context
-  begin
-
-  private lemma aux1:
-    assumes "\<forall>x\<in>passed. \<not> a \<preceq> x"
-        and "passed \<subseteq> Collect reachable"
-        and "reachable a"
-    shows "
-    ((insert a passed, wait', brk'),
-     passed, wait, brk)
-    \<in> worklist_var"
-  proof -
-    from assms have "a \<notin> passed" by auto
-    with assms(2,3) show ?thesis
-    by (auto simp: worklist_inv_def worklist_var_def finite_psupset_def)
-  qed
-
-  private lemma aux2:
+  lemma worklist_algo_list_inv_ref:
+    fixes x x'
     assumes
-      "a' \<in> passed"
-      "a \<preceq> a'"
-      "wait = a # wait'"
-      "worklist_inv_frontier passed wait"
-    shows "worklist_inv_frontier passed wait'"
-    using assms unfolding worklist_inv_frontier_def
-    using trans
-    apply clarsimp
-    by (metis (no_types, lifting) Un_iff count_eq_zero_iff count_single mset_contains_eq mset_un_cases)
+      "\<not> F a\<^sub>0" "\<not> F a\<^sub>0"
+      "(x, x') \<in> {((passed,wait,brk), (passed',wait',brk')). passed = passed' \<and> mset wait = wait' \<and> brk = brk' }"
+      "worklist_inv x'"
+    shows "worklist_inv_list x"
+    using assms
+    unfolding worklist_inv_def worklist_inv_list_def
+    unfolding worklist_inv_frontier_def worklist_inv_frontier_list_def
+    unfolding start_subsumed_def start_subsumed_list_def
+    by auto
 
-  private lemma aux5:
-    assumes
-      "a' \<in> passed"
-      "a \<preceq> a'"
-      "wait = a # wait'"
-      "start_subsumed passed wait"
-    shows "start_subsumed passed wait'"
-    using assms unfolding start_subsumed_def apply clarsimp
-    by (metis Un_iff insert_DiffM2 local.trans mset_right_cancel_elem)
+  lemma take_from_list_take_from_mset_ref[refine]:
+    "take_from_list xs \<le> \<Down> {((x, xs),(y, m)). x = y \<and> mset xs = m} (take_from_mset m)"
+    if "mset xs = m"
+    using that unfolding take_from_list_def take_from_mset_def
+    by (clarsimp simp: pw_le_iff refine_pw_simps)
 
-  (* XXX Move to misc *)
-  (* XXX Unused *)
-  lemma mset_remove_member:
-    "x \<in># A - B" if "x \<in># A" "x \<notin># B"
-    using that
-    by (metis count_greater_zero_iff in_diff_count not_in_iff)
+  lemma add_succ_spec_list_add_succ_spec_ref[refine]:
+    "add_succ_spec_list xs b \<le> \<Down> {((xs, b), (m, b')). mset xs = m \<and> b = b'} (add_succ_spec m b')"
+    if "mset xs = m" "b = b'"
+    using that unfolding add_succ_spec_list_def add_succ_spec_def
+    by (clarsimp simp: pw_le_iff refine_pw_simps)
 
-  private lemma aux3:
-    assumes
-      "set wait \<subseteq> Collect reachable"
-      "wait = a # wait''"
-      "\<forall> s \<in> set wait'' \<union> Collect (E a). \<exists> s' \<in> set wait'. s \<preceq> s'"
-      "worklist_inv_frontier passed wait"
-    shows "worklist_inv_frontier (insert a passed) wait'"
-  proof -
-    from assms(1,2) have "reachable a"
-      by (simp add: subset_iff)
-    with finitely_branching have [simp, intro!]: "finite (Collect (E a))" .
-
-    show ?thesis unfolding worklist_inv_frontier_def
-      apply safe
-      subgoal
-        using assms by auto
-      subgoal for b b'
-      proof -
-        assume A: "E b b'" "b \<in> passed"
-        with assms obtain b'' where b'': "b'' \<in> passed \<union> set wait" "b' \<preceq> b''"
-          unfolding worklist_inv_frontier_def by blast
-        from this(1) show ?thesis
-          apply standard
-          subgoal
-            using \<open>b' \<preceq> b''\<close> by auto
-          subgoal
-            apply (cases "a = b''")
-            subgoal
-              using b''(2) by blast
-            subgoal premises prems
-            proof -
-              from prems \<open>wait = _\<close> have "b'' \<in> set wait''"
-                by simp
-              with assms prems \<open>b' \<preceq> b''\<close> show ?thesis
-                by (blast intro: local.trans)
-            qed
-            done
-          done
-      qed
-      done
-  qed
-
-  private lemma aux6:
-    assumes
-      "wait = a # wait''"
-      "start_subsumed passed wait"
-      "\<forall> s \<in> set (tl wait) \<union> Collect (E a). \<exists> s' \<in> set wait'. s \<preceq> s'"
-    shows "start_subsumed (insert a passed) wait'"
-    using assms unfolding start_subsumed_def by (auto dest: trans)
-
-  lemma empty_E_star:
-    "empty x'" if "E\<^sup>*\<^sup>* x x'" "reachable x" "empty x"
-    using that unfolding reachable_def
-    by (induction rule: converse_rtranclp_induct)
-       (blast intro: empty_E[unfolded reachable_def] rtranclp.rtrancl_into_rtrancl)+
-
-  lemma aux4:
-    assumes "worklist_inv_frontier passed []" "reachable x" "start_subsumed passed []"
-            "passed \<subseteq> Collect reachable"
-    shows "\<exists> x' \<in> passed. x \<preceq> x'"
-  proof -
-    from \<open>reachable x\<close> have "E\<^sup>*\<^sup>* a\<^sub>0 x" by (simp add: reachable_def)
-    from assms(3) obtain b where "a\<^sub>0 \<preceq> b" "b \<in> passed" unfolding start_subsumed_def by auto
-    have "\<exists>x'. \<exists> x''. E\<^sup>*\<^sup>* b x' \<and> x \<preceq> x' \<and> x' \<preceq> x'' \<and> x'' \<in> passed" if
-                      "E\<^sup>*\<^sup>* a x" "a \<preceq> b"    "b \<preceq> b'"  "b' \<in> passed"
-                      "reachable a" "reachable b" for a b b'
-    using that proof (induction arbitrary: b b' rule: converse_rtranclp_induct)
-      case base
-      then show ?case by auto
-    next
-      case (step a a1 b b')
-      show ?case
-      proof (cases "empty a")
-        case True
-        with step.prems step.hyps have "empty x" by - (rule empty_E_star, auto)
-        with step.prems show ?thesis by (auto intro: empty_subsumes)
-      next
-        case False
-        with \<open>E a a1\<close> \<open>a \<preceq> b\<close> \<open>reachable a\<close> \<open>reachable b\<close> obtain b1 where
-          "E b b1" "a1 \<preceq> b1"
-        using mono by blast
-       then obtain b1' where "E b' b1'" "b1 \<preceq> b1'"
-          using False empty_mono assms(4) mono step.prems by blast
-        with \<open>b' \<in> passed\<close> assms(1) obtain b1'' where "b1'' \<in> passed" "b1' \<preceq> b1''"
-        unfolding worklist_inv_frontier_def by auto
-        with \<open>b1 \<preceq> _\<close> have "b1 \<preceq> b1''" using trans by blast
-        with step.IH[OF \<open>a1 \<preceq> b1\<close> this \<open>b1'' \<in> passed\<close>] \<open>reachable a\<close> \<open>E a a1\<close> \<open>reachable b\<close> \<open>E b b1\<close>
-        obtain x' x'' where
-          "E\<^sup>*\<^sup>* b1 x'" "x \<preceq> x'" "x' \<preceq> x''" "x'' \<in> passed"
-        by (auto intro: step_reachable)
-        moreover from \<open>E b b1\<close> \<open>E\<^sup>*\<^sup>* b1 x'\<close> have "E\<^sup>*\<^sup>* b x'" by auto
-        ultimately show ?thesis by auto
-      qed
-    qed
-    from this[OF \<open>E\<^sup>*\<^sup>* a\<^sub>0 x\<close> \<open>a\<^sub>0 \<preceq> b\<close> refl \<open>b \<in> _\<close>] assms(4) \<open>b \<in> passed\<close> show ?thesis
-    by (auto intro: trans)
-  qed
-
-  theorem worklist_algo_correct:
-    "worklist_algo \<le> SPEC (\<lambda> brk. brk \<longleftrightarrow> F_reachable)"
-  proof -
-    note [simp] = size_Diff_submset pred_not_lt_is_zero
-    note [dest] = set_mset_mp
-    show ?thesis
-    unfolding worklist_algo_def add_succ_spec_def F_reachable_def
-      apply (refine_vcg wf_worklist_var)
-      (* F a\<^sub>0*)
-      apply (auto; fail) []
-      (* Invar start*)
-      apply (auto simp: worklist_inv_def worklist_inv_frontier_def start_subsumed_def; fail)
-      (* Precondition for take-from-set *)
-      apply (simp; fail)
-      (* State is subsumed by passed*)
-        (* Assertion *)
-        apply (auto simp: worklist_inv_def; fail)
-        (*Invariant*)
-        apply (auto simp: worklist_inv_def aux2 aux5
-              dest: in_diffD
-              split: if_split_asm; fail)
-        (*Variant*)
-        apply (auto simp: worklist_inv_def worklist_var_def intro: finite_subset[OF _ finite_reachable]; fail)
-
-      (* Insert successors to wait *)
-        (*Invariant*)
-        apply (clarsimp split: if_split_asm) (* Split on F in successors *)
-          (* Found final state *)
-          apply (clarsimp simp: worklist_inv_def; blast intro: step_reachable; fail)
-          (* No final state *)
-      apply (auto
-        simp: worklist_inv_def aux3[rotated 3] aux6 finitely_branching step_reachable
-        dest: in_diffD)[]
-        (*Variant*)
-        apply (auto simp: worklist_inv_def aux1; fail)
-      (* I \<and> \<not>b \<Longrightarrow> post *)
-      using F_mono apply (fastforce simp: worklist_inv_def dest!: aux4)
-      done
-  qed
-
-  lemmas [refine_vcg] = worklist_algo_correct[THEN order_trans]
-
-  end -- \<open>Context\<close>
+  lemma worklist_algo_list_ref[refine]: "worklist_algo_list \<le> \<Down>Id worklist_algo"
+    unfolding worklist_algo_list_def worklist_algo_def
+    apply (refine_rcg)
+               apply blast
+              prefer 2
+              apply (rule worklist_algo_list_inv_ref; assumption)
+    by auto
 
 end -- \<open>Search Space\<close>
-
 
 subsection \<open>Towards an Implementation\<close>
 locale Worklist1_Defs = Search_Space_Defs +
@@ -404,9 +159,12 @@ begin
       (wait,False)"
     unfolding add_succ1_def filter_insert_wait_def by (intro HOL.eq_reflection HOL.refl)
 
-  lemma add_succ1_ref[refine]: "\<lbrakk>(wait,wait')\<in>Id; (a,a')\<in>b_rel Id reachable\<rbrakk> \<Longrightarrow> add_succ1 wait a \<le> \<Down>(Id \<times>\<^sub>r bool_rel) (add_succ_spec wait' a')"
+  lemma add_succ1_ref[refine]:
+    "add_succ1 wait a \<le> \<Down>(Id \<times>\<^sub>r bool_rel) (add_succ_spec_list wait' a')"
+    if "(wait,wait')\<in>Id" "(a,a')\<in>b_rel Id reachable"
+    using that
     apply simp
-    unfolding add_succ_spec_def add_succ1_def
+    unfolding add_succ_spec_list_def add_succ1_def
     apply (refine_vcg nfoldli_rule[where I = "\<lambda>l1 _ (wait',brk). if brk then \<exists>a'. E a a' \<and> F a' else set wait' \<subseteq> set wait \<union> set l1 \<and> set l1 \<inter> Collect F = {} \<and> (\<forall> x \<in> set wait \<union> set l1. \<exists> x' \<in> set wait'. x \<preceq> x')"])
     apply (auto; fail)
     using succs_correct[of a] apply (auto; fail)
@@ -423,7 +181,7 @@ begin
         else do {
           let passed = {};
           let wait = [a\<^sub>0];
-          (passed, wait, brk) \<leftarrow> WHILEIT worklist_inv (\<lambda> (passed, wait, brk). \<not> brk \<and> wait \<noteq> [])
+          (passed, wait, brk) \<leftarrow> WHILEIT worklist_inv_list (\<lambda> (passed, wait, brk). \<not> brk \<and> wait \<noteq> [])
             (\<lambda> (passed, wait, brk). do
               {
                 (a, wait) \<leftarrow> take_from_list wait;
@@ -442,15 +200,21 @@ begin
       }
     "
 
-  lemma worklist_algo1_ref[refine]: "worklist_algo1 \<le> \<Down>Id worklist_algo"
-    unfolding worklist_algo1_def worklist_algo_def
+  lemma worklist_algo1_list_ref[refine]: "worklist_algo1 \<le> \<Down>Id worklist_algo_list"
+    unfolding worklist_algo1_def worklist_algo_list_def
     apply (refine_rcg)
     apply refine_dref_type
     unfolding worklist_inv_def
     apply auto
     done
 
-end
+  lemma worklist_algo1_ref[refine]: "worklist_algo1 \<le> \<Down>Id worklist_algo"
+  proof -
+    note worklist_algo1_list_ref
+    also note worklist_algo_list_ref
+    finally show ?thesis .
+  qed
 
+end -- \<open>Worklist1\<close>
 
 end -- \<open>Theory\<close>
